Rename files, prepare for generalized security labels

specification/Dynamics.v
@@ -8,9 +8,6 @@ Inductive tm : Type :=
 | tm_un : tm -> tm
 | tm_let : string -> tm -> tm -> tm.
 
-Inductive ty : Type :=
-| Pub : ty
-| Sec : ty.
 
 Fixpoint subst (x : string) (s : nat) (t : tm) : tm :=
   match t with
@@ -45,5 +42,22 @@ Fixpoint lookup {A} (m : list (string * A)) (x : string) : option A :=
       else lookup m' x
   end.
 
-  
-  
+
+Axiom f_un : nat -> nat.
+Axiom f_bin : nat -> nat -> nat.
+
+Inductive big_eval : tm -> nat -> Prop := 
+| Etm_val : forall v,
+  big_eval (tm_val v) v
+| Etm_un : forall e v v',
+  big_eval e v -> v' = f_un v -> 
+  big_eval (tm_un e) v'
+| Etm_bin : forall e1 e2 v1 v2 v,
+  big_eval e1 v1 -> 
+  big_eval e2 v2 -> 
+  v = f_bin v1 v2 -> 
+  big_eval (tm_bin e1 e2) v
+| Etm_let : forall x e1 e2 v1 v2,
+  big_eval e1 v1 -> 
+  big_eval (subst x v1 e2) v2 -> 
+  big_eval (tm_let x e1 e2) v2.
